verif/btrees/verif_splitnode_part1.v
@@ -35,7 +35,7 @@ Lemma splitnode_main_if_part2_proof:
          (H3 : Zlength allent_end = Fanout + 1 - fri)
          (FRIRANGE : 0 <= fri <= Fanout)
          (H5 : key_repr ke = key_repr k)
-         (H4 : 0 <= fri < Zlength (le_to_list (nth_first_le le fri) ++ allent_end))
+         (H4 : 0 <= fri < Zlength (map entry_val_rep (le_to_list (nth_first_le le fri)) ++ allent_end))
          (FRILENGTH : Zlength (le_to_list (nth_first_le le fri)) = fri),
 semax (func_tycontext f_splitnode Vprog Gprog [])
   (EX ent_end : list (val * (val + val)),
@@ -49,10 +49,9 @@ semax (func_tycontext f_splitnode Vprog Gprog [])
    btnode_rep (empty_node true false Last vnewnode);
    data_at Ews tentry (Vptrofs (Ptrofs.repr (k_ k)), inr xe) pe;
    data_at Tsh (tarray tentry 16)
-     (le_to_list (nth_first_le le fri) ++
-      (Vptrofs (Ptrofs.repr (k_ k)),
-      inr (force_val (sem_cast_pointer xe)))
-      :: le_to_list (suble fri Fanout le) ++ ent_end) v_allEntries;
+     (map entry_val_rep (le_to_list (nth_first_le le fri)) ++
+      (Vptrofs (Ptrofs.repr (k_ k)), inr (force_val (sem_cast_pointer xe)))
+      :: map entry_val_rep (le_to_list (suble fri Fanout le)) ++ ent_end) v_allEntries;
    entry_rep (keyval val ke ve xe))) splitnode_main_if_part2
   (frame_ret_assert
      (function_body_ret_assert tvoid
@@ -94,7 +93,11 @@ Proof.
            lvar _allEntries (tarray tentry 16) v_allEntries; temp _node nval; temp _entry pe)
     SEP (mem_mgr gv; btnode_rep (splitnode_left n e); btnode_rep (empty_node true false Last vnewnode);
          data_at Ews tentry (Vptrofs (Ptrofs.repr (k_ k)), inr xe) pe;
-         data_at Tsh (tarray tentry 16) (le_to_list (nth_first_le le fri) ++ (Vptrofs (Ptrofs.repr (k_ k)), inr (force_val (sem_cast_pointer xe))) :: le_to_list (suble fri Fanout le) ++ ent_end) v_allEntries; le_iter_sepcon (skipn_le (insert_le le e) Middle))).
+         data_at Tsh (tarray tentry 16) 
+            (map entry_val_rep (le_to_list (nth_first_le le fri)) 
+             ++ (Vptrofs (Ptrofs.repr (k_ k)), inr (force_val (sem_cast_pointer xe))) 
+              :: map entry_val_rep (le_to_list (suble fri Fanout le)) ++ ent_end) v_allEntries;
+          le_iter_sepcon (skipn_le (insert_le le e) Middle))).
     {                           (* fri < 8 *)
       Intros.
       unfold Sfor.              (* both forward_loop and forward_for_simple_bound fail here *)
@@ -111,20 +114,21 @@ SEP (mem_mgr gv; le_iter_sepcon (nth_first_le (insert_le le e) Middle);
        (Val.of_bool false,
        (Vint (Int.repr 8),
        (optionally getval nullval ptr0,
-        le_to_list (nth_first_le (insert_le le e) i) ++ le_end))))) nval;
+        map entry_val_rep (le_to_list (nth_first_le (insert_le le e) i)) ++ le_end))))) nval;
      optionally btnode_rep emp ptr0; btnode_rep (empty_node true false Last vnewnode);
      data_at Ews tentry (Vptrofs (Ptrofs.repr (k_ k)), inr xe) pe;
      data_at Tsh (tarray tentry 16)
-       (le_to_list (nth_first_le le fri) ++
+       (map entry_val_rep (le_to_list (nth_first_le le fri)) ++
         (Vptrofs (Ptrofs.repr (k_ k)), inr (force_val (sem_cast_pointer xe)))
-        :: le_to_list (suble fri Fanout le) ++ ent_end) v_allEntries))%assert.
+        :: map entry_val_rep (le_to_list (suble fri Fanout le)) ++ ent_end) v_allEntries))%assert.
       - Exists fri.
-        Exists (le_to_list(skipn_le le fri) ++ ent_end0).
+        Exists (map entry_val_rep (le_to_list(skipn_le le fri)) ++ ent_end0).
         entailer!.
         set (fri := findRecordIndex n k) in *.
         rewrite le_split with (i:=fri) (le:=le) at 1.
         rewrite le_to_list_app.
         replace (nth_first_le (insert_le le e) fri) with (nth_first_le le fri).
+        rewrite map_app.
         rewrite app_assoc. cancel.
         rewrite insert_fri with (fri:=fri) (key0:=ke).
         rewrite nth_first_app_same1. auto.
@@ -136,9 +140,12 @@ SEP (mem_mgr gv; le_iter_sepcon (nth_first_le (insert_le le e) Middle);
         Intros i.
         Intros le_end.             
         forward_if.
-        + assert(HINSERT: (le_to_list (nth_first_le le fri) ++ (Vptrofs (Ptrofs.repr (k_ k)), inr (force_val (sem_cast_pointer xe))) :: le_to_list (suble fri Fanout le) ++ ent_end) = le_to_list (insert_le le e) ++ ent_end).
+        + assert(HINSERT: (map entry_val_rep (le_to_list (nth_first_le le fri)) 
+                                      ++ (Vptrofs (Ptrofs.repr (k_ k)), inr (force_val (sem_cast_pointer xe)))
+                                        :: map entry_val_rep (le_to_list (suble fri Fanout le)) ++ ent_end) 
+                       = map entry_val_rep (le_to_list (insert_le le e)) ++ ent_end).
           { rewrite insert_fri with (fri:=fri) (key0:=ke).
-            rewrite le_to_list_app.
+            rewrite le_to_list_app, map_app.
             simpl. rewrite H5.
             rewrite suble_skip. unfold key_repr.
             rewrite <- app_assoc. simpl.
@@ -165,15 +172,15 @@ SEP (mem_mgr gv; le_iter_sepcon (nth_first_le (insert_le le e) Middle);
               rewrite H0. rep_omega. }
             rewrite HENTRY. simpl entry_rep. entailer!. }
           rename H11 into XIPTR.
-          assert(HZNTH: forall ent_end, Znth (d:=(Vundef,inl Vundef)) i (le_to_list (insert_le le e) ++ ent_end) = entry_val_rep (keyval val ki vi xi)).
-          { intros. apply Znth_to_list. auto. }
+          assert(HZNTH: forall ent_end, Znth (d:=(Vundef,inl Vundef)) i (map entry_val_rep (le_to_list (insert_le le e)) ++ ent_end) = entry_val_rep (keyval val ki vi xi)).
+          { intros. apply Znth_to_list'. auto. }
           assert(0 <= i < 8) by omega.
           assert_PROP(Zlength le_end > 0).
           { entailer!.
             clear - H14 H11 H0. simplify_value_fits in H14.
             destruct H14, H1, H2, H3, H4.
             simplify_value_fits in H5. destruct H5.
-            rewrite Zlength_app in H5. rewrite le_to_list_length in H5.
+            rewrite Zlength_app, Zlength_map in H5. rewrite le_to_list_length in H5.
             rewrite numKeys_nth_first in H5. omega.
             simpl in H0. rewrite numKeys_le_insert. rewrite H0. rep_omega.  }            
           rename H12 into LEEND.
@@ -192,21 +199,27 @@ SEP (mem_mgr gv; le_iter_sepcon (nth_first_le (insert_le le e) Middle);
           rewrite upd_Znth_twice.
           rewrite upd_Znth_same.
           rewrite upd_Znth_app2.
+          rewrite !Zlength_map.
           rewrite le_to_list_length.
           rewrite numKeys_nth_first.
           replace(i-i) with 0 by omega.
           rewrite upd_Znth0. fold (Z.succ i).
           rewrite nth_first_increase with (e:=(keyval val ki vi xi)).
-          rewrite le_to_list_app. simpl. rewrite <- app_assoc.
+          rewrite le_to_list_app. simpl. rewrite map_app, <- app_assoc.
           cancel.
           auto.
           rewrite numKeys_le_insert. simpl in H0. rewrite H0. rep_omega.
+          rewrite !Zlength_map.
           rewrite le_to_list_length. rewrite numKeys_nth_first. rep_omega.
           rewrite numKeys_le_insert. simpl in H0. rewrite H0. rep_omega.
-          rewrite Zlength_app. rewrite le_to_list_length. rewrite numKeys_nth_first.
+          rewrite Zlength_app.
+          rewrite !Zlength_map.
+          rewrite le_to_list_length. rewrite numKeys_nth_first.
           omega.
           rewrite numKeys_le_insert. simpl in H0. rewrite H0. rep_omega.
-          rewrite Zlength_app. rewrite le_to_list_length. rewrite numKeys_nth_first.
+          rewrite Zlength_app.
+          rewrite !Zlength_map.
+          rewrite le_to_list_length. rewrite numKeys_nth_first.
           omega.
           rewrite numKeys_le_insert. simpl in H0. rewrite H0. rep_omega.
         + 
@@ -232,8 +245,8 @@ SEP (mem_mgr gv; le_iter_sepcon (nth_first_le (insert_le le e) Middle);
       { rewrite le_split with (i:=Middle) at 1. rewrite le_to_list_app. auto.
         simpl in H0. rewrite H0. rewrite Middle_eq, Fanout_eq. omega. }
       rewrite SPLITLE.
-      rewrite <- app_assoc.
-      Exists (le_to_list (skipn_le le Middle) ++ ent_end0).
+      rewrite map_app, <- app_assoc.
+      Exists (map entry_val_rep (le_to_list (skipn_le le Middle)) ++ ent_end0).
       simpl. rewrite numKeys_nth_first.
       rewrite nth_first_insert with (k:=ke). cancel.
       unfold e. simpl. auto.
@@ -245,9 +258,12 @@ SEP (mem_mgr gv; le_iter_sepcon (nth_first_le (insert_le le e) Middle);
     }
     rewrite unfold_btnode_rep with (n:=empty_node true false Last vnewnode).
     simpl. Intros ent_empty.
-    assert(HINSERT: (le_to_list (nth_first_le le fri) ++ (Vptrofs (Ptrofs.repr (k_ k)), inr xe) :: le_to_list (suble fri Fanout le) ++ ent_end) = le_to_list (insert_le le e) ++ ent_end).
+    assert(HINSERT: (map entry_val_rep (le_to_list (nth_first_le le fri))
+                              ++ (Vptrofs (Ptrofs.repr (k_ k)), inr xe)
+                               :: map entry_val_rep (le_to_list (suble fri Fanout le)) ++ ent_end) 
+                            = map entry_val_rep (le_to_list (insert_le le e)) ++ ent_end).
     { rewrite insert_fri with (fri:=fri) (key0:=ke).
-      rewrite le_to_list_app.
+      rewrite le_to_list_app, map_app.
       simpl. rewrite H5.
       rewrite suble_skip. unfold key_repr.
       unfold n in H0. simpl in H0. rewrite <- app_assoc. simpl.
@@ -265,9 +281,11 @@ SEP (mem_mgr gv; le_iter_sepcon (nth_first_le (insert_le le e) Middle);
      SEP (mem_mgr gv; btnode_rep (splitnode_left n e);
      malloc_token Ews tbtnode vnewnode;
      data_at Ews tbtnode
-       (Vtrue, (Vfalse, (Val.of_bool Last, (Vint (Int.repr 0), (nullval, le_to_list(suble Middle i (insert_le le e)) ++ ent_right))))) vnewnode;
+       (Vtrue, (Vfalse, (Val.of_bool Last, (Vint (Int.repr 0), (nullval,
+        map entry_val_rep (le_to_list(suble Middle i (insert_le le e))) ++ ent_right)))))
+       vnewnode;
      data_at Ews tentry (Vptrofs (Ptrofs.repr (k_ k)), inr xe) pe;
-     data_at Tsh (tarray tentry 16) (le_to_list (insert_le le e) ++ ent_end) v_allEntries;
+     data_at Tsh (tarray tentry 16) (map entry_val_rep (le_to_list (insert_le le e)) ++ ent_end) v_allEntries;
      le_iter_sepcon (skipn_le (insert_le le e) Middle))))%assert.                             
     
     { entailer!. rewrite suble_nil. Exists ent_empty. entailer!.
@@ -293,8 +311,8 @@ SEP (mem_mgr gv; le_iter_sepcon (nth_first_le (insert_le le e) Middle);
           rewrite H0. rep_omega.  }
         rewrite HENTRY. simpl entry_rep. entailer!. }
       rename H9 into XIPTR.
-      assert(HZNTH: forall ent_end, Znth (d:=(Vundef,inl Vundef)) i (le_to_list (insert_le le e) ++ ent_end) = entry_val_rep (keyval val ki vi xi)).
-      { intros. apply Znth_to_list. auto. }
+      assert(HZNTH: forall ent_end, Znth (d:=(Vundef,inl Vundef)) i (map entry_val_rep (le_to_list (insert_le le e)) ++ ent_end) = entry_val_rep (keyval val ki vi xi)).
+      { intros. apply Znth_to_list'. auto. }
 
       forward.                  (* t'18=allEntries[i]->key *)
       apply prop_right; rep_omega.
@@ -318,12 +336,13 @@ SEP (mem_mgr gv; le_iter_sepcon (nth_first_le (insert_le le e) Middle);
       rewrite upd_Znth_twice by list_solve.
       rewrite upd_Znth_same by list_solve.
       rewrite upd_Znth_app2.
+      rewrite !Zlength_map.
       rewrite le_to_list_length.
       rewrite numKeys_suble.
       simpl. replace (i - 8 - (i - Middle)) with 0 by rep_omega.
       rewrite upd_Znth0. fold (Z.succ i).
       rewrite suble_increase with (e:=(keyval val ki vi xi)).
-      rewrite le_to_list_app. simpl. rewrite <- app_assoc.
+      rewrite le_to_list_app. simpl. rewrite map_app, <- app_assoc.
       cancel.
 
       rep_omega.
@@ -331,6 +350,7 @@ SEP (mem_mgr gv; le_iter_sepcon (nth_first_le (insert_le le e) Middle);
       auto.
       rep_omega.
       rewrite numKeys_le_insert. simpl in H0. rewrite H0. rep_omega.
+      rewrite !Zlength_map.
       rewrite le_to_list_length. rewrite numKeys_suble. rep_omega.
       rep_omega. 
       rewrite numKeys_le_insert. simpl in H0. rewrite H0. rep_omega. 
@@ -362,7 +382,7 @@ SEP (mem_mgr gv; le_iter_sepcon (nth_first_le (insert_le le e) Middle);
       rewrite H0. rep_omega. } 
     destruct NTHENTRY as [emid NTHENTRY].
     assert(HZNTH: nth_entry_le Middle (insert_le le e) = Some emid) by auto.
-    eapply Znth_to_list with (endle:=ent_end) in HZNTH.
+    apply Znth_to_list' with (endle:=ent_end) in HZNTH.
     rewrite Middle_eq in HZNTH. simpl in HZNTH.
     
     forward.                    (* t'16=allEntries[8]->key *)
